Further refactor lemmas etc

Escallon/Chomsky_Normal_Form_Fun/Chomsky_Normal_Form_Fun.thy
@@ -40,7 +40,7 @@ lemma replace_tm_length_unchanged[simp]:
   
 
 lemma replace_tm_id_iff_tm_notin_syms:
-  assumes "replace_tm A sms = (t,sms')"
+  assumes "replace_tm A sms = (t_opt,sms')"
   shows "(\<forall>t. Tm t \<notin> set sms) \<longleftrightarrow> sms = sms'"
   using assms by (induction sms arbitrary: sms') (auto split: sym.splits prod.splits)
 
@@ -48,23 +48,29 @@ lemma replace_tm_id_iff_tm_notin_syms:
 (*Proofs break with iff lemma. Fix?*)
 lemma tm_notin_syms_impl_replace_tm_id:
   assumes "\<forall>t. Tm t \<notin> set sms" 
-          "replace_tm A sms = (t,sms')"
+          "replace_tm A sms = (t_opt,sms')"
   shows "sms = sms'"
   using assms replace_tm_id_iff_tm_notin_syms by fast
-lemma replace_tm_id_impl_tm_notin_syms:
-  assumes "replace_tm A sms = (t,sms)" 
+lemma replace_tm_id_impl_no_tms:
+  assumes "replace_tm A sms = (t_opt,sms)" 
   shows "\<forall>t. Tm t \<notin> set sms"
   using assms replace_tm_id_iff_tm_notin_syms by fast
 
-lemma replace_tm_none_impl_id:
-  shows "replace_tm A sms = (None,sms') \<Longrightarrow> sms = sms'"
+lemma replace_tm_none_iff_id:
+  "replace_tm A sms = (t_opt,sms') \<Longrightarrow> t_opt = None \<longleftrightarrow> sms = sms'"
   by (induction sms arbitrary: sms')(auto split: sym.splits prod.splits)
+
+corollary no_tms_impl_id:
+  assumes "\<forall>t. Tm t \<notin> set sms"
+  shows "replace_tm A sms = (None,sms)"
+  using assms tm_notin_syms_impl_replace_tm_id replace_tm_none_iff_id 
+  by (metis old.prod.exhaust)
 
 lemma replace_tm_not_id_impl_some:
   assumes "replace_tm A sms = (t_opt,sms')"
           "sms \<noteq> sms'"
         obtains t where "t_opt = Some t"
-  using assms replace_tm_none_impl_id option.exhaust by metis
+  using assms replace_tm_none_iff_id option.exhaust by metis
 
 lemma replace_tm_some_impl_not_id:
   assumes "replace_tm A sms = (Some t,sms')"
@@ -108,34 +114,70 @@ fun uniformize_fun :: "['n::infinite, ('n,'t) prods, ('n,'t) prods] \<Rightarrow
   "uniformize_fun S ps0 ((l,r) # ps) = 
     (let A = fresh (nts ps0 \<union> {S}) in case replace_tm A r of
     (None,_) \<Rightarrow> uniformize_fun S ps0 ps |
-    (Some t, r') \<Rightarrow> if r = r' \<or> length r < 2 then uniformize_fun S ps0 ps
+    (Some t, r') \<Rightarrow> if length r < 2 then uniformize_fun S ps0 ps
       else (removeAll (l,r) ps0) @ [(A, [Tm t]), (l,r')])"
 
 lemma uniformize_fun_id:
-  assumes "\<forall>(l,r)\<in>set ps. Tm t \<notin> set r \<or> length r < 2"
-  shows "uniformize_fun A t ps0 ps = ps0"
-  using assms tm_notin_syms_impl_replace_tm_id by (induction ps) fastforce+
+  "\<forall>(l,r)\<in>set ps. (\<forall>t. Tm t \<notin> set r) \<or> length r < 2 \<Longrightarrow> uniformize_fun S ps0 ps = ps0"
+proof (induction ps)
+  case (Cons p ps)
+  have "uniformize_fun S ps0 (p#ps) = uniformize_fun S ps0 ps" 
+  proof -
+    let ?A = "fresh (nts ps0 \<union> {S})"
+    obtain l r where p_def: "p = (l,r)" by fastforce
+    with Cons(2) consider (tm_free) "\<forall>t. Tm t \<notin> set r" | (len_ub) "length r < 2" by auto
+    then show ?thesis 
+    proof cases
+      case tm_free
+      then have "replace_tm ?A r = (None,r)" 
+        using no_tms_impl_id by metis
+      then show ?thesis using p_def by simp
+    next
+      case len_ub
+      consider r'   where "replace_tm ?A r = (None,r')" | 
+               t r' where "replace_tm ?A r = (Some t,r')"
+        using option.exhaust by (metis old.prod.exhaust)
+      then show ?thesis by cases (use len_ub p_def in auto)
+    qed
+  qed
+  then show ?case using Cons by simp
+qed (fastforce split: prod.splits)
+
+lemma len_lt_2_impl_uniformize_fun_rec:
+  assumes "length r < 2"
+  shows "uniformize_fun S ps0 ((l,r)#ps) = uniformize_fun S ps0 ps"
+proof -
+  let ?A = "fresh (nts ps0 \<union> {S})"
+  consider r' where   "replace_tm ?A r = (None,r')" |
+           r' t where "replace_tm ?A r = (Some t,r')"
+    using option.exhaust old.prod.exhaust by metis
+   then show ?thesis by cases (use assms in auto)
+qed
+  
 
 lemma uniformize_fun_uniform_prepend:
-   "\<forall>(l,r)\<in>set xs. Tm t \<notin> set r \<or> length r < 2 \<Longrightarrow>
-    uniformize_fun A t ps0 (xs@ps) = uniformize_fun A t ps0 ps"
+   "\<forall>(l,r)\<in>set xs. (\<forall>t. Tm t \<notin> set r) \<or> length r < 2 \<Longrightarrow>
+    uniformize_fun S ps0 (xs@ps) = uniformize_fun S ps0 ps"
 proof (induction xs)
   case (Cons x xs)
   then obtain l r where lr_def: "x = (l,r)" by auto
-  hence "uniformize_fun A t ps0 ((x#xs)@ps) = uniformize_fun A t ps0 ((l,r)#xs@ps)" by simp
-  also have "... = uniformize_fun A t ps0 (xs@ps)"
+  hence "uniformize_fun S ps0 ((x#xs)@ps) = uniformize_fun S ps0 ((l,r)#xs@ps)" by simp
+  also have "... = uniformize_fun S ps0 (xs@ps)"
   proof -
-    from Cons(2) lr_def have "Tm t \<notin> set r \<or> length r < 2" by simp
-    hence "replace_tm A t r = r \<or> length r < 2" using tm_notin_syms_impl_replace_tm_id by fast
-    thus ?thesis by auto
+    let ?A = "fresh (nts ps0 \<union> {S})"
+    from Cons(2) lr_def have "(\<forall>t. Tm t \<notin> set r) \<or> length r < 2" by simp
+    hence "replace_tm ?A r = (None,r) \<or> length r < 2" using no_tms_impl_id by fast 
+    then consider (id) "replace_tm ?A r = (None,r)" | (len_ub) "length r < 2" by blast
+    thus ?thesis by cases (fastforce split: prod.splits,
+                           use len_lt_2_impl_uniformize_fun_rec in simp)
   qed
-  also have "... = uniformize_fun A t ps0 ps" using Cons by simp
+  also have "... = uniformize_fun S ps0 ps" using Cons by simp
   finally show ?case .
 qed simp
 
 lemma uniformize_fun_ps0_uniform_app:
   assumes "\<forall>(l,r)\<in>set xs. Tm t \<notin> set r \<or> length r < 2"
-  shows "uniformize_fun A t (xs@ys) ps = xs @ uniformize_fun A t ys ps"
+  shows "uniformize_fun S (xs@ys) ps = xs @ uniformize_fun S ys ps"
 proof (induction ps)
   case (Cons p ps)
   then obtain l r where lr_def: "p = (l,r)" 
@@ -146,24 +188,25 @@ proof (induction ps)
   proof cases
     case not_unif
     with assms(1) lr_def have p_notin_xs: "p \<notin> set xs" by auto
-    from not_unif lr_def have "uniformize_fun A t (xs@ys) (p#ps) 
-                      = removeAll p (xs@ys) @ [(A, [Tm t]), (l,replace_tm A t r)]" 
+    let ?A = "fresh (nts (xs@ys) \<union> {S})"
+    from not_unif lr_def have "uniformize_fun S (xs@ys) (p#ps) 
+                      = removeAll p (xs@ys) @ [(?A, [Tm t]), (l,replace_tm ?A r)]" 
       by (smt (verit) replace_tm_id_iff_tm_notin_syms uniformize_fun.simps(2)
           verit_comp_simplify1(3))
     also have "... = xs @ removeAll p ys @ [(A, [Tm t]), (l,replace_tm A t r)]"
       using p_notin_xs by simp
     also have "... = xs @ uniformize_fun A t ys (p#ps)" using not_unif 
-      by (smt (verit) lr_def replace_tm_id_impl_tm_notin_syms
+      by (smt (verit) lr_def replace_tm_id_impl_no_tms
           uniformize_fun.simps(2) verit_comp_simplify1(3))
     finally show ?thesis .
   next
     case unif
     hence unif_ite: "replace_tm A t r = r \<or> length r < 2" using tm_notin_syms_impl_replace_tm_id 
       by fast
-    with lr_def have "uniformize_fun A t (xs@ys) (p#ps) = uniformize_fun A t (xs@ys) ps" 
+    with lr_def have "uniformize_fun S (xs@ys) (p#ps) = uniformize_fun S (xs@ys) ps" 
       by fastforce
-    also have "... = xs @ uniformize_fun A t ys ps" using Cons .
-    also have "... = xs @ uniformize_fun A t ys (p#ps)" using unif_ite lr_def by fastforce
+    also have "... = xs @ uniformize_fun S ys ps" using Cons .
+    also have "... = xs @ uniformize_fun S ys (p#ps)" using unif_ite lr_def by fastforce
     finally show ?thesis .
   qed
 qed simp
@@ -201,7 +244,7 @@ using assms proof (induction ps arbitrary: thesis)
   next
     case fst
     hence "r0 \<noteq> replace_tm A t r0" find_theorems name:replace_tm
-      using replace_tm_id_impl_tm_notin_syms by metis
+      using replace_tm_id_impl_no_tms by metis
     with fst lr0_def show ?thesis using Cons(2)[of _ _ "[]"] by simp
   qed
 qed simp
@@ -232,9 +275,8 @@ proof -
 qed
 
 lemma uniformize_fun_is_uniformized:
-  assumes "uniformize_fun A t ps ps \<noteq> ps"
-          "A = fresh (nts ps \<union> {S})"
-  shows "uniformize A t S ps (uniformize_fun A t ps ps)"
+  assumes "uniformize_fun S ps ps \<noteq> ps"
+  shows "uniformize S ps (uniformize_fun S ps ps)"
 proof -
   from assms obtain l r q s  where lr_in_ps: "(l,r) \<in> set ps"
                           and replace_neq: "r \<noteq> replace_tm A t r"
